Formulate some POPLmark monotonicity and weakeing laws with respect to context enequalities.

theories/Morphisms.v
@@ -3,14 +3,30 @@ Require Import Autosubst.Basics Autosubst.Classes Autosubst.Decidable.
 
 Axiom prop_ext : Coq.Logic.ClassicalFacts.prop_extensionality.
 
+(* JK: level and assoc ok? *)
+(* Domain of a relation *)
+Notation "'DOM' R" := (R >> @ex _) (at level 56, right associativity).
+(* Lifting functions to relations *)
+Notation "'REL' f" := (f >> @eq _) (at level 56, right associativity).
+
 Definition subset {A : Type} (P1 P2 : A -> Prop) := forall a, P1 a -> P2 a.
+Notation "P :c Q" := (subset P Q) (at level 57, right associativity).
 
 Lemma subset_eq {A : Type} (x : A) P : subset (eq x) P <-> P x.
 Proof. split; repeat intro; subst; eauto. Qed.
 
-Definition rsubset {A B : Type} (R1 R2 : A -> B -> Prop) := forall a b, R1 a b -> R2 a b.
+Lemma subset_refl {A : Type} (P : A -> Prop) : subset P P.
+Proof. firstorder. Qed.
 
-Lemma rsubset_scons {A : Type} (P1 P2 : A -> Prop) R1 R2 : rsubset (P1 .: R1) (P2 .: R2) <-> subset P1 P2 /\ rsubset R1 R2.
+Lemma subset_trans {A : Type} (P1 P2 P3 : A -> Prop) :
+  subset P1 P2 -> subset P2 P3 -> subset P1 P3.
+Proof. firstorder. Qed.
+
+Definition rsubset {A B : Type} (R1 R2 : A -> B -> Prop) := forall a b, R1 a b -> R2 a b.
+Notation "R :< S" := (rsubset R S) (at level 57, right associativity).
+
+Lemma rsubset_scons {A : Type} (P1 P2 : A -> Prop) R1 R2 :
+  P1 .: R1 :< P2 .: R2  <-> P1 :c P2 /\ R1 :< R2.
 Proof.
   split.
   - intros H. split.
@@ -19,6 +35,18 @@ Proof.
   - intros [H1 H2] [|n]; simpl; eauto.
 Qed.
 
+(* JK: may require improvement *)
+Lemma rsubset_subset {A B : Type} (R1 R2 : A -> B -> Prop): R1 :< R2 -> (DOM R1) :c (DOM R2).
+Proof. firstorder. Qed.
+
+(* JK: may require improvement *)
+Lemma rsubset_refl {A B : Type} (R : A -> B -> Prop): R :< R.
+Proof. firstorder. Qed.
+
+Lemma rsubset_trans {A B : Type} (R1 R2 R3 : A -> B -> Prop) :
+  R1 :< R2 -> R2 :< R3 -> R1 :<  R3.
+Proof. firstorder. Qed.
+
 (* Definition papp {A B : Type} (R : A -> B -> Prop) P : B -> Prop := fun b => exists a, P a /\ R a b. *)
 
 Definition rapp {A B : Type} (R : A -> B -> Prop) P : B -> Prop := fun b => exists a, P a /\ R a b.
@@ -26,7 +54,7 @@ Definition rapp {A B : Type} (R : A -> B -> Prop) P : B -> Prop := fun b => exis
 Lemma rapp_eq1 {A : Type} : rapp eq = @id (A -> Prop).
 Proof. repeat(f_ext; intro). apply prop_ext. firstorder. now subst. Qed.
 
-Lemma rapp_eq_app {A B : Type} (f g : A -> B) (P : A -> Prop) x : f x = g x -> P x -> rapp (f >> eq) P (g x).
+Lemma rapp_eq_app {A B : Type} (f g : A -> B) (P : A -> Prop) x : f x = g x -> P x -> rapp (REL f) P (g x).
 Proof. firstorder. Qed.
 
 Lemma rapp_eq2 (A B : Type) (R : A -> B -> Prop) x : rapp R (eq x) = R x.
@@ -35,8 +63,15 @@ Proof. f_ext. intros. apply prop_ext. firstorder congruence. Qed.
 Lemma rapp_rapp {A B C : Type} (R1 : A -> B -> Prop) (R2 : B -> C -> Prop) : rapp R1 >> rapp R2 = rapp (R1 >> rapp R2).
 Proof. (repeat (f_ext; intros)). apply prop_ext. firstorder. Qed.
 
-Lemma rapp_ex (A B : Type) (f : A -> B) : rapp (f >> eq) >> @ex _ = @ex _.
+Lemma rapp_ex (A B : Type) (f : A -> B) : DOM rapp (REL f) = @ex A.
 Proof. f_ext. intros. apply prop_ext. unfold rapp. simpl. firstorder eauto. Qed.
+
+Definition total {A B : Type} (R : A -> B -> Prop) := forall a : A, exists b : B, R a b. (* Depr. *)
+
+(* JK: may require improvement *)
+Lemma sub_rapp_ex {A B C : Type} (R1 : A -> B -> Prop) (R2 : B -> C -> Prop) :
+  (DOM (R1 >> rapp R2)) :c (DOM R1).
+Proof. firstorder. Qed.
 
 Lemma ex_True {A : Type} y : (exists x : A, y = x) = True.
 Proof. apply prop_ext. intuition. now eexists. Qed.
@@ -48,6 +83,49 @@ Definition rcomp {A B C : Type} (R1 : A -> B -> Prop) (R2 : B -> C -> Prop) : A 
   R1 >> rapp R2.
 
 (* Lemma rcomp_cons {A B : Type} x f (R : A -> B -> Prop) : rcomp (P .: R1) R2 = P .: f >> R. *)
+
+(* JK: may require improvement *)
+Lemma rsubset_rcomp {A B C : Type} (R1 R1' : A -> B -> Prop) (R2 R2' : B -> C -> Prop) :
+  R1 :< R1' -> R2 :< R2' -> R1 >> rapp R2 :< R1' >> rapp R2'.
+Proof. firstorder. Qed.
+
+(* Converse relation; maybe deprecated ...  *)
+Definition conv {A B : Type} (R : A -> B -> Prop) := fun b a => R a b.
+
+Lemma rapp_conv {A B : Type} (f : A -> B) :
+  rapp (conv (REL f)) = fun P => f >> P.
+Proof. repeat (f_ext; intro). apply prop_ext. cbv. firstorder. congruence. Qed.
+
+Definition injectiveF {A B : Type} (f : A -> B) := forall a1 a2 : A, f a1 = f a2 -> a1 = a2.
+
+(* JK: this law requires injectivity of f ... *)
+(* Lemma conv_eq {A B : Type} (f : A -> B) (a : A) : *)
+(*   injectiveF f -> conv (f >> eq) (f a) = eq a. *)
+(* Proof. intros f_inj. f_ext. intros. cbv. apply prop_ext. firstorder; auto. congruence. Qed. *)
+
+Lemma conv_fun_subset {A B : Type} (f : A -> B) (a : A) :
+  eq a :c conv (REL f) (f a).
+Proof. intros a' Ea; congruence. Qed.
+
+Definition surjectiveR {A B : Type} (R : A -> B -> Prop) := forall b : B, exists a : A, R a b.
+
+Lemma conv_total {A B : Type} (R : A -> B -> Prop) : surjectiveR R -> total (conv R).
+Proof. firstorder. Qed.
+
+Definition functional {A B : Type} (R : A -> B -> Prop) := forall a b b', R a b -> R a b' -> b = b'.
+
+Lemma fun_func {A B : Type} (f : A -> B) : functional (REL f).
+Proof. intros a b b'. simpl. congruence. Qed.
+
+Lemma preconv_K1 {A B : Type} (R : A-> B -> Prop) : functional R -> conv R >> rapp R :< eq.
+Proof. firstorder. Qed.
+
+(* Lemma convK1 {A B : Type} (R : A -> B -> Prop) : *)
+(*   surjectiveR R -> functional R -> (conv R) >> rapp R = eq. *)
+(* Proof. *)
+(*   intros R_surj R_fun. unfold conv. f_ext. intros b. f_ext. intros b'. apply prop_ext. firstorder eauto. *)
+(*   simpl. subst. destruct (R_surj b') as [a Ha]. firstorder. *)
+(* Qed. *)
 
 Section SubstInstance.
 
